Auto/Embedding/LamPrep.lean
@@ -1,0 +1,191 @@
+import Auto.Embedding.LamConv
+
+namespace Auto.Embedding.Lam
+
+theorem eq_not_of_ne (h : a ≠ b) : a = (¬ b) :=
+  propext (Iff.intro
+    (fun ha hb => h (Eq.trans (eq_true ha) (eq_true hb).symm))
+    (fun nb => Classical.byContradiction (fun na => h (Eq.trans (eq_false na) (eq_false nb).symm))))
+
+theorem ne_of_eq_not (h : a = (¬ b)) : a ≠ b := fun h' =>
+  have hb : b := Classical.byContradiction (fun nb => nb (Eq.mp h' (Eq.mp h.symm nb)))
+  have hnb : ¬ b := Eq.mp h (Eq.mp h'.symm hb)
+  hnb hb
+
+def LamTerm.equalize (t : LamTerm) : LamTerm := .mkEq (.base .prop) t (.base .trueE)
+
+theorem LamEquiv.not_true_equiv_false :
+  LamEquiv lval lctx (.base .prop) (.mkNot (.base .trueE)) (.base .falseE) := by
+  exists LamWF.mkNot (.ofBase .ofTrueE); exists LamWF.ofBase .ofFalseE; intro lctxTerm
+  dsimp [LamWF.interp, LamBaseTerm.LamWF.interp, notLift]
+  apply GLift.down.inj; dsimp; apply eq_false; exact fun h => (h .intro)
+
+theorem LamEquiv.prop_ne_equiv_eq_not
+  (wfl : LamWF lval.toLamTyVal ⟨lctx, lhs, .base .prop⟩)
+  (wfr : LamWF lval.toLamTyVal ⟨lctx, rhs, .base .prop⟩) :
+  LamEquiv lval lctx (.base .prop) (.mkNot (.mkEq (.base .prop) lhs rhs)) (.mkEq (.base .prop) lhs (.mkNot rhs)) := by
+  exists LamWF.mkNot (LamWF.mkEq wfl wfr); exists LamWF.mkEq wfl (.mkNot wfr); intro lctxTerm
+  dsimp [LamWF.interp, LamBaseTerm.LamWF.interp, notLift, eqLiftFn]
+  apply GLift.down.inj; apply propext (Iff.intro ?mp ?mpr)
+  case mp =>
+    intro h; apply GLift.down.inj; apply eq_not_of_ne
+    intro h'; apply h; apply GLift.down.inj _ _ h'
+  case mpr =>
+    intro h h'; have h' := _root_.congrArg GLift.down h'; revert h'
+    apply ne_of_eq_not; dsimp at h; rw [h]
+
+theorem LamTerm.maxEVarSucc_equalize : (LamTerm.equalize t).maxEVarSucc = t.maxEVarSucc := by
+  dsimp [maxEVarSucc]; simp [Nat.max, Nat.max_zero_left, Nat.max_zero_right]
+
+theorem LamEquiv.equalize (wft : LamWF lval.toLamTyVal ⟨lctx, t, .base .prop⟩) :
+  LamEquiv lval lctx (.base .prop) t t.equalize := by
+  dsimp [LamTerm.equalize]; exists wft; exists (.mkEq wft (.ofBase .ofTrueE))
+  intro lctxTerm; apply GLift.down.inj
+  apply propext (Iff.intro
+    (fun h => GLift.down.inj _ _ (eq_true h))
+    (fun h => of_eq_true (_root_.congrArg GLift.down h)))
+
+theorem LamThmEquiv.equalize (wft : LamThmWF lval lctx (.base .prop) t) :
+  LamThmEquiv lval lctx (.base .prop) t t.equalize :=
+  fun lctx' => LamEquiv.equalize (wft lctx')
+
+def LamTerm.true_eq_false_equiv_false? (t : LamTerm) : Option LamTerm :=
+  match t.beq (.mkEq (.base .prop) (.base .trueE) (.base .falseE)) with
+  | true => .some (.base .falseE)
+  | false => .none
+
+theorem LamTerm.maxEVarSucc_true_eq_false_equiv_false?
+  (heq : LamTerm.true_eq_false_equiv_false? t = .some t') :
+  t'.maxEVarSucc = t.maxEVarSucc := by
+  dsimp [LamTerm.true_eq_false_equiv_false?] at heq; revert heq
+  cases hbeq : t.beq (.mkEq (.base .prop) (.base .trueE) (.base .falseE))
+  case true =>
+    intro h; cases h; cases (LamTerm.eq_of_beq_eq_true hbeq)
+    dsimp [maxEVarSucc]; rfl
+  case false =>
+    intro h; cases h
+
+theorem LamEquiv.true_eq_false_equiv_false?
+  (wft : LamWF lval.toLamTyVal ⟨lctx, t, s⟩)
+  (heq : LamTerm.true_eq_false_equiv_false? t = .some t') :
+  LamEquiv lval lctx (.base .prop) t t' := by
+  dsimp [LamTerm.true_eq_false_equiv_false?] at heq; revert heq
+  cases hbeq : t.beq (.mkEq (.base .prop) (.base .trueE) (.base .falseE))
+  case true =>
+    intro h; cases h; cases (LamTerm.eq_of_beq_eq_true hbeq)
+    cases wft.getFn.getFn.getBase; exists wft
+    match wft with
+    | .ofApp _ (.ofApp _ (.ofBase (.ofEq _)) (.ofBase .ofTrueE)) (.ofBase .ofFalseE) =>
+      exists (.ofBase .ofFalseE); intro lctxTerm; apply GLift.down.inj
+      dsimp [LamWF.interp, LamBaseTerm.LamWF.interp, eqLiftFn]
+      apply propext (Iff.intro ?mp False.elim)
+      case mp =>
+        intro h; have h' := GLift.up.inj h; contradiction
+  case false =>
+    intro h; cases h
+
+theorem LamThmEquiv.true_eq_false_equiv_false?
+  (wft : LamThmWF lval lctx s t)
+  (heq : LamTerm.true_eq_false_equiv_false? t = .some t') :
+  LamThmEquiv lval lctx (.base .prop) t t' :=
+  fun lctx' => LamEquiv.true_eq_false_equiv_false? (wft lctx') heq
+
+def LamTerm.false_eq_true_equiv_false? (t : LamTerm) : Option LamTerm :=
+  match t.beq (.mkEq (.base .prop) (.base .falseE) (.base .trueE)) with
+  | true => .some (.base .falseE)
+  | false => .none
+
+theorem LamTerm.maxEVarSucc_false_eq_true_equiv_false?
+  (heq : LamTerm.false_eq_true_equiv_false? t = .some t') :
+  t'.maxEVarSucc = t.maxEVarSucc := by
+  dsimp [LamTerm.false_eq_true_equiv_false?] at heq; revert heq
+  cases hbeq : t.beq (.mkEq (.base .prop) (.base .falseE) (.base .trueE))
+  case true =>
+    intro h; cases h; cases (LamTerm.eq_of_beq_eq_true hbeq)
+    dsimp [maxEVarSucc]; rfl
+  case false =>
+    intro h; cases h
+
+theorem LamEquiv.false_eq_true_equiv_false?
+  (wft : LamWF lval.toLamTyVal ⟨lctx, t, s⟩)
+  (heq : LamTerm.false_eq_true_equiv_false? t = .some t') :
+  LamEquiv lval lctx (.base .prop) t t' := by
+  dsimp [LamTerm.false_eq_true_equiv_false?] at heq; revert heq
+  cases hbeq : t.beq (.mkEq (.base .prop) (.base .falseE) (.base .trueE) )
+  case true =>
+    intro h; cases h; cases (LamTerm.eq_of_beq_eq_true hbeq)
+    cases wft.getFn.getFn.getBase; exists wft
+    match wft with
+    | .ofApp _ (.ofApp _ (.ofBase (.ofEq _)) (.ofBase .ofFalseE)) (.ofBase .ofTrueE) =>
+      exists (.ofBase .ofFalseE); intro lctxTerm; apply GLift.down.inj
+      dsimp [LamWF.interp, LamBaseTerm.LamWF.interp, eqLiftFn]
+      apply propext (Iff.intro ?mp False.elim)
+      case mp =>
+        intro h; have h' := GLift.up.inj h; contradiction
+  case false =>
+    intro h; cases h
+
+theorem LamThmEquiv.false_eq_true_equiv_false?
+  (wft : LamThmWF lval lctx s t)
+  (heq : LamTerm.false_eq_true_equiv_false? t = .some t') :
+  LamThmEquiv lval lctx (.base .prop) t t' :=
+  fun lctx' => LamEquiv.false_eq_true_equiv_false? (wft lctx') heq
+
+def LamTerm.ne_true_equiv_eq_false? (t : LamTerm) : Option LamTerm :=
+  match t with
+  | .app _ (.base .not) (.app s (.app _ (.base (.eq _)) lhs) (.base .trueE)) =>
+    .some (.app s (.app s (.base (.eq s)) lhs) (.base .falseE))
+  | _ => .none
+
+theorem LamTerm.maxEVarSucc_ne_true_equiv_eq_false?
+  (heq : LamTerm.ne_true_equiv_eq_false? t = .some t') :
+  t'.maxEVarSucc = t.maxEVarSucc := by
+  cases t <;> try cases heq
+  case app s fn arg =>
+    cases fn <;> try cases heq
+    case base b =>
+      cases b <;> try cases heq
+      cases arg <;> try cases heq
+      case app _ fn arg =>
+        cases fn <;> try cases heq
+        case app _ fn' arg' =>
+          cases fn' <;> try cases heq
+          case base b =>
+            cases b <;> try cases heq
+            cases arg <;> try cases heq
+            case base b =>
+              cases b <;> try cases heq
+              simp [maxEVarSucc, Nat.max]
+              simp [Nat.max_zero_left, Nat.max_zero_right]
+
+theorem LamEquiv.ne_true_equiv_eq_false?
+  (wft : LamWF lval.toLamTyVal ⟨lctx, t, s⟩)
+  (heq : LamTerm.ne_true_equiv_eq_false? t = .some t') :
+  LamEquiv lval lctx (.base .prop) t t' := by
+  cases t <;> try cases heq
+  case app s fn arg =>
+    cases fn <;> try cases heq
+    case base b =>
+      cases b <;> try cases heq
+      cases wft.getFn.getBase
+      cases arg <;> try cases heq
+      case app _ fn arg =>
+        cases fn <;> try cases heq
+        case app _ fn' arg' =>
+          cases fn' <;> try cases heq
+          case base b =>
+            cases b <;> try cases heq
+            cases arg <;> try cases heq
+            case base b =>
+              cases b <;> try cases heq
+              match wft with
+              | .ofApp _ (.ofBase .ofNot) (.ofApp _ (.ofApp _ (.ofBase (.ofEq _)) Hlhs) (.ofBase .ofTrueE)) =>
+                apply LamEquiv.trans (prop_ne_equiv_eq_not Hlhs (.ofBase .ofTrueE))
+                apply LamEquiv.congrArg (.ofApp _ (.ofBase (.ofEq _)) Hlhs)
+                apply LamEquiv.not_true_equiv_false
+
+theorem LamThmEquiv.ne_true_equiv_eq_false?
+  (wft : LamThmWF lval lctx s t)
+  (heq : LamTerm.ne_true_equiv_eq_false? t = .some t') :
+  LamThmEquiv lval lctx (.base .prop) t t' :=
+  fun lctx' => LamEquiv.ne_true_equiv_eq_false? (wft lctx') heq
